# baseURI: https://datamodel.terra.bio/TerraCore
# imports: https://datamodel.terra.bio/TerraCoreValueSets
# imports: https://datamodel.terra.bio/TerraDCAT_ap
# imports: https://datamodel.terra.bio/imports/EFO_subset
# imports: https://datamodel.terra.bio/imports/NCBITaxon_Organisms_subset
# imports: https://datamodel.terra.bio/imports/OBIAssay_subset
# imports: https://datamodel.terra.bio/imports/OBI_core
# prefix: TerraCore

@prefix : <https://datamodel.terra.bio/TerraCore#> .
@prefix NCBITaxon_Organisms: <https://datamodel.terra.bio/NCBITaxon_Organisms_subset#> .
@prefix OBIAssay: <https://datamodel.terra.bio/OBIAssay_subset#> .
@prefix TerraCore: <https://datamodel.terra.bio/TerraCore#> .
@prefix TerraCoreValueSets: <https://datamodel.terra.bio/TerraCoreValueSets#> .
@prefix TerraDCAT_ap: <https://datamodel.terra.bio/TerraDCAT_ap#> .
@prefix dc: <http://purl.org/dc/elements/1.1/> .
@prefix dcat: <http://www.w3.org/ns/dcat#> .
@prefix dct: <http://purl.org/dc/terms/> .
@prefix duo: <http://purl.obolibrary.org/obo/duo-basic.owl#> .
@prefix nsf2_full_mtg: <http://www.jcvi.org/framework/nsf2_full_mtg#> .
@prefix obo: <http://purl.obolibrary.org/obo/> .
@prefix oboInOwl: <http://www.geneontology.org/formats/oboInOwl#> .
@prefix owl: <http://www.w3.org/2002/07/owl#> .
@prefix prov: <http://www.w3.org/ns/prov#> .
@prefix rdf: <http://www.w3.org/1999/02/22-rdf-syntax-ns#> .
@prefix rdfs: <http://www.w3.org/2000/01/rdf-schema#> .
@prefix skos: <http://www.w3.org/2004/02/skos/core#> .
@prefix xsd: <http://www.w3.org/2001/XMLSchema#> .

obo:BFO_0000001
  owl:equivalentClass prov:Entity ;
.
prov:Agent
  owl:equivalentClass dct:Agent ;
.
prov:Entity
  owl:equivalentClass obo:BFO_0000001 ;
.

<https://datamodel.terra.bio/TerraCore>
  a owl:Ontology ;
  dc:contributor "Sid Cox" ;
  dc:creator "Kathy Reinold" ;
  dct:date "20 Jul 2020" ;
  dct:license <https://github.com/DataBiosphere/terra-interoperability-model/blob/master/LICENSE> ;
  rdfs:comment "Please cite The Broad Institute of Harvard and MIT, Data Sciences Platform." ;
  owl:imports <https://datamodel.terra.bio/TerraCoreValueSets> ;
  owl:imports <https://datamodel.terra.bio/TerraDCAT_ap> ;
  owl:imports <https://datamodel.terra.bio/imports/EFO_subset> ;
  owl:imports <https://datamodel.terra.bio/imports/NCBITaxon_Organisms_subset> ;
  owl:imports <https://datamodel.terra.bio/imports/OBIAssay_subset> ;
  owl:imports <https://datamodel.terra.bio/imports/OBI_core> ;
  owl:versionInfo "Version 1.0.0" ;
.































































































































TerraCore:id
  a owl:DatatypeProperty ;
  rdfs:comment "This value can be used as a reference from other objects within the same information system (i.e. primary and foreign keys), and it should be unique per type of object.  Contrast with \\\"business identifiers\\\" which are assigned outside the information system and are captured as cross references." ;
  rdfs:domain prov:Entity ;
  rdfs:label "id" ;
  rdfs:range [
      owl:unionOf (
          xsd:anyURI
          xsd:string
        ) ;
    ] ;
  skos:definition "The information system-specific identifier of the entity in the context in which it is being referenced. The same data object copied to a different system will likely have a different \\\\\\\"id\\\\\\\" in the new system since \\\\\\\"id\\\\\\\" values are system specific and do not represent persistent cross-system business identifiers. Additional equivalent identifiers are captured as cross references." ;
  skos:prefLabel "id" ;
.











TerraDCAT_ap:DataCollection
  rdfs:subClassOf [
      a owl:Restriction ;
      owl:cardinality "1"^^xsd:nonNegativeInteger ;
      owl:onProperty TerraCore:id ;
    ] ;
.
TerraDCAT_ap:DataSnapshot
  rdfs:subClassOf [
      a owl:Restriction ;
      owl:cardinality "1"^^xsd:nonNegativeInteger ;
      owl:onProperty TerraCore:id ;
    ] ;
.
TerraDCAT_ap:Dataset
  rdfs:subClassOf [
      a owl:Restriction ;
      owl:cardinality "1"^^xsd:nonNegativeInteger ;
      owl:onProperty TerraCore:id ;
    ] ;
  rdfs:subClassOf [
      a owl:Restriction ;
      owl:minCardinality "1"^^xsd:nonNegativeInteger ;
      owl:onProperty dcat:contactPoint ;
    ] ;
  rdfs:subClassOf [
      a owl:Restriction ;
      owl:minCardinality "1"^^xsd:nonNegativeInteger ;
      owl:onProperty TerraCore:hasDataModality ;
    ] ;
  rdfs:subClassOf [
      a owl:Restriction ;
      owl:minCardinality "1"^^xsd:nonNegativeInteger ;
      owl:onProperty TerraDCAT_ap:hasDataUsePermission ;
    ] ;
  rdfs:subClassOf [
      a owl:Restriction ;
      owl:minCardinality "1"^^xsd:nonNegativeInteger ;
      owl:onProperty TerraDCAT_ap:hasOwner ;
    ] ;
.
TerraDCAT_ap:hasConsentGroup
  TerraCore:hasColumnLabel "consent_group" ;
.
TerraDCAT_ap:hasDataUseModifier
  TerraCore:hasColumnLabel "data_use_modifier" ;
.
TerraDCAT_ap:hasDataUsePermission
  TerraCore:hasColumnLabel "data_use_permission" ;
.
TerraDCAT_ap:hasOriginalPublication
  TerraCore:hasColumnLabel "original_publication" ;
.
TerraDCAT_ap:hasOwner
  TerraCore:hasColumnLabel "owner" ;
.
TerraDCAT_ap:hasPrincipalInvestigator
  rdfs:range [
      owl:unionOf (
          xsd:string
          TerraCore:PrincipalInvestigator
        ) ;
    ] ;
  TerraCore:hasColumnLabel "principal_investigator" ;
.
TerraDCAT_ap:hasRegisteredIdentifier
  TerraCore:hasColumnLabel "registered_id" ;
.
